imp/Imp2CsharpminorMatch.v
@@ -105,8 +105,8 @@ Section MATCH.
       EventsL.interp_Es (ModSemL.prog ms)
                         (transl_all mn (` x0 : val <- (let (_, retv) := v in Ret retv);; Ret (Any.upcast x0))) st1);; Ret (snd x0).
 
-  Definition itree_of_cont_stmt efs (s : Imp.stmt) :=
-    fun ge le ms mn rp => itree_of_imp_cont (denote_stmt efs s) ge le ms mn rp.
+  Definition itree_of_cont_stmt (s : Imp.stmt) :=
+    fun ge le ms mn rp => itree_of_imp_cont (denote_stmt s) ge le ms mn rp.
 
   Definition imp_state := itree eventE Any.t.
   Definition imp_cont {T} {R} := (r_state * p_state * (lenv * T)) -> itree eventE (r_state * p_state * (lenv * R)).
@@ -118,7 +118,8 @@ Section MATCH.
   (* next block of src's initialized genv *)
   Definition src_init_nb : Imp.programL -> nat := fun src => int_len src.
   (* next block of tgt's initialized genv *)
-  Definition tgt_init_nb : Imp.programL -> Values.block := fun src => Pos.of_succ_nat (2 + (ext_len src) + (int_len src)).
+  Definition tgt_init_len := List.length (init_g ++ c_sys).
+  Definition tgt_init_nb : Imp.programL -> Values.block := fun src => Pos.of_succ_nat (tgt_init_len + (ext_len src) + (int_len src)).
 
   Definition get_sge (src : Imp.programL) := Sk.load_skenv (Sk.sort (ImpMod.get_modL src).(ModL.sk)).
   Definition get_tge (tgt : Csharpminor.program) := Genv.globalenv tgt.
@@ -130,7 +131,7 @@ Section MATCH.
     fun src blk =>
       match (compile src) with
       | OK tgt =>
-        if (ge_dec blk (src_init_nb src)) then Pos.of_succ_nat (2 + (ext_len src) + blk)
+        if (ge_dec blk (src_init_nb src)) then Pos.of_succ_nat (tgt_init_len + (ext_len src) + blk)
         else
           let sg := get_sge src in
           let tg := get_tge tgt in
@@ -181,7 +182,6 @@ Section MATCH.
   Definition ret_call_main := Kseq exit_stmt Kstop.
 
   (* global env is fixed when src program is fixed *)
-  Variable efs : extFuns.
   Variable ge : SkEnv.t.
   (* ModSem should be fixed with src too *)
   Variable ms : ModSemL.t.
@@ -196,7 +196,7 @@ Section MATCH.
   | match_code_cont
       code itr ktr chead ctail
       (CST: compile_stmt code = chead)
-      (ITR: itr = fun '(r, p, (le, _)) => itree_of_cont_stmt efs code ge le ms mn (r, p))
+      (ITR: itr = fun '(r, p, (le, _)) => itree_of_cont_stmt code ge le ms mn (r, p))
       (MCONT: match_code mn ktr ctail)
     :
       match_code mn (fun x => (itr x >>= ktr)) (chead :: ctail)
@@ -248,7 +248,7 @@ Section MATCH.
       (WFCONT: wf_ccont tcont)
       (MCONT: match_code mn next (get_cont_stmts tcont))
       (MSTACK: @match_stack sz src mn stack (get_cont_stack tcont))
-      (ITR: itr = itree_of_cont_stmt efs code ge le ms mn (rstate, pstate))
+      (ITR: itr = itree_of_cont_stmt code ge le ms mn (rstate, pstate))
     :
       match_states src (x <- itr;; next x >>= stack) (State tf tcode tcont empty_env tle tm)
   .
